

## Finite Diff Approach 1.2)

equation:  $\frac{d^2 y}{dx^2} + \alpha \frac{dy}{dx} + \beta y = f(x)$

BC:  $y(a) = y_a$   $y(b) = y_b$

finite diff.

$$\left. \frac{dy}{dx} \right|_i = \frac{y_{i+1} - y_{i-1}}{2h}$$

$$\left. \frac{d^2 y}{dx^2} \right|_i = \frac{y_{i+1} - 2y_i + y_{i-1}}{h^2}$$

$$\Rightarrow \frac{y_{i+1} - 2y_i + y_{i-1}}{h^2} + \alpha \cdot \frac{y_{i+1} - y_{i-1}}{2h} + \beta y_i = f(x_i)$$

rearrange and multiply by  $h^2$

$$y_{i+1} \left(1 + \frac{h}{2}\alpha\right) + y_i (h^2\beta - 2) + y_{i-1} \left(1 - \frac{h}{2}\alpha\right) = h^2 f(x_i)$$

In case of the assignment:

Question 1.2:

$$\frac{d^2 \phi^*}{dx^{*2}} = \phi^*(x^*)$$

domain =  $0 < y < 10$

Boundary condition:

$$- \phi^*(0) = \frac{\phi_0}{v_T}$$

$$- \frac{d\phi^*}{dx^*}(x^* = 10) = 0$$

where  $\phi^* = \frac{\phi}{v_T}$  with  $\phi = \phi_0 \cdot \exp\left(-\frac{x}{\lambda}\right)$

Centralized Diff method:

$$\frac{1 \cdot \phi^*[i+1] - 2 \cdot \phi^*[i] + 1 \cdot \phi^*[i-1]}{h^2} = \phi^*(x^*)[i]$$

rearrange:  $1 \cdot \phi^*[i+1] - 2 \cdot \phi^*[i] + 1 \cdot \phi^*[i-1] = 0$

$$\phi^*[i+1] - (2+h^2)\phi^*[i] + \phi^*[i-1] = 0$$

notice it is in range  $[1, N-2]$

Constructing matrix A:  $(A y = b)$

case  $i=1$ :  $\phi_{i-1}^* = \phi^*(0) = \frac{\phi_0}{v_T}$

$$1 \cdot \phi^*(0) - (2+h^2)\phi^*[1] + \phi^*[i-1] = 0$$

$$- (2+h^2)\phi^*[1] + \phi^*[i-1] = 0 - 1 \cdot \phi^*(0)$$

case  $2 \leq i \leq N-3$

$$1 \cdot \phi^*[i-1] - (2+h^2)\phi^*[i] + \phi^*[i-1] = 0$$

case  $i = N-2$  : (far right case)

Neumann boundary:

$$\frac{d\phi^*}{dx^*} = 0$$

$$\Rightarrow \frac{\phi[i] - \phi[i-2]}{2h} = 0 \Rightarrow \phi[i] = \phi[i-2]$$

in matrix A:

$$1 \cdot \phi[i-2] - (2+h^2) \phi[i-1] + 1 \cdot \phi[i] = 0$$

plug in for  $\phi[i] = \phi[i-2]$

$$\Rightarrow 2 \phi[i-2] - (2+h^2) \phi[i-1] = 0$$

Question 2:

$$\frac{d^2 \phi}{dx^2} = \frac{q_0 e}{\epsilon} \sinh\left(\frac{e\phi(x)}{k_B T}\right)$$

$$\frac{d^2 \phi^*}{dx^{*2}} = \sinh(\phi^*(x^*))$$

$$x^* = \frac{x}{\lambda} \quad \phi^* = \frac{\phi}{V_T} \quad V_T = \frac{k_B T}{e}$$

$$\frac{1 \cdot \phi^*[i-1] - 2 \cdot \phi^*[i] + 1 \cdot \phi^*[i+1]}{h^2} = \sinh(\phi^*(x^*))$$

$$1 \cdot \phi^*[i-1] - 2 \cdot \phi^*[i] - h^2 \sinh(\phi^*[i]) + 1 \cdot \phi^*[i+1] = 0$$

$f(x) \rightarrow$  can be solved with Newton Raphson

where Newton Raphson will guess for the value of  $\phi^*$ . It does so by expanding F around an estimate  $\phi[i]$  using Taylor series:

making a the Jacobian:

$$F(\phi[i] + \delta\phi) \approx F(\phi[i]) + J(\phi[i]) \cdot \delta\phi$$

$\hat{=}$  Jacobian

$$F[i] = \phi[i-1] - 2\phi[i] - h^2 \sinh(\phi[i]) + \phi[i+1]$$

Term:  $\phi[i-1]$

Derivative:  $\frac{dF_i}{d\phi[i-1]} = 1$

note any other derivative = 0  
 $\Rightarrow$  only diagonal has values

$\phi[i]$

$$\frac{dF_i}{d\phi[i]} = -2 - h^2 \cosh(\phi[i])$$

$\phi[i+1]$

$$\frac{dF_i}{d\phi[i+1]} = 1$$

note only Neumann conditions must be applied to the Jacobian

the Dirichlet boundary  $\phi[0] = \phi_{i=0}/V_T$  will be defined in solution

however Neumann must be defined

$$\therefore @ N = -1 \quad \frac{d\phi^*}{dx^*} = 0 \Rightarrow$$

$$F[N-1] = 2\phi[i-2] - 2\phi[i-1] - h^2 \cosh(\phi[i-1])$$